ldir-lean/.lake/build/ir/LDIRProofs/ProofLayoutProperties.c
@@ -144,6 +144,23 @@ LEAN_EXPORT lean_object* lp_LDIRProofs_LDIR_totalDemerits(lean_object*, lean_obj
 LEAN_EXPORT lean_object* lp_LDIRProofs_LDIR_totalDemerits___boxed(lean_object*, lean_object*);
 LEAN_EXPORT lean_object* lp_LDIRProofs_LDIR_kp__findOptimalBreaks(lean_object*);
 LEAN_EXPORT lean_object* lp_LDIRProofs_LDIR_kp__findOptimalBreaks___boxed(lean_object*);
+LEAN_EXPORT lean_object* lp_LDIRProofs_LDIR_lineWidth;
+lean_object* lean_nat_add(lean_object*, lean_object*);
+LEAN_EXPORT lean_object* lp_LDIRProofs_List_foldl___at___00LDIR_cumWidth_spec__0(lean_object*, lean_object*);
+LEAN_EXPORT lean_object* lp_LDIRProofs_List_foldl___at___00LDIR_cumWidth_spec__0___boxed(lean_object*, lean_object*);
+lean_object* lean_mk_empty_array_with_capacity(lean_object*);
+static lean_once_cell_t lp_LDIRProofs_LDIR_cumWidth___closed__0_once = LEAN_ONCE_CELL_INITIALIZER;
+static lean_object* lp_LDIRProofs_LDIR_cumWidth___closed__0;
+lean_object* l___private_Init_Data_List_Impl_0__List_takeTR_go___redArg(lean_object*, lean_object*, lean_object*, lean_object*);
+LEAN_EXPORT lean_object* lp_LDIRProofs_LDIR_cumWidth(lean_object*, lean_object*);
+lean_object* lean_nat_sub(lean_object*, lean_object*);
+LEAN_EXPORT uint8_t lp_LDIRProofs_LDIR_feasibleBreak(lean_object*, lean_object*, lean_object*);
+LEAN_EXPORT lean_object* lp_LDIRProofs_LDIR_feasibleBreak___boxed(lean_object*, lean_object*, lean_object*);
+static lean_once_cell_t lp_LDIRProofs_LDIR_demeritsReal___closed__0_once = LEAN_ONCE_CELL_INITIALIZER;
+static lean_object* lp_LDIRProofs_LDIR_demeritsReal___closed__0;
+LEAN_EXPORT lean_object* lp_LDIRProofs_LDIR_demeritsReal(lean_object*, lean_object*, lean_object*);
+LEAN_EXPORT lean_object* lp_LDIRProofs___private_LDIRProofs_ProofLayoutProperties_0__LDIR_instReprKPItem_repr_match__1_splitter___redArg(lean_object*, lean_object*, lean_object*, lean_object*);
+LEAN_EXPORT lean_object* lp_LDIRProofs___private_LDIRProofs_ProofLayoutProperties_0__LDIR_instReprKPItem_repr_match__1_splitter(lean_object*, lean_object*, lean_object*, lean_object*, lean_object*);
 LEAN_EXPORT lean_object* lp_LDIRProofs_LDIR_KPItem_ctorIdx(lean_object* x_1) {
 _start:
 {
@@ -1097,6 +1114,251 @@ lean_dec(x_1);
 return x_2;
 }
 }
+static lean_object* _init_lp_LDIRProofs_LDIR_lineWidth(void) {
+_start:
+{
+lean_object* x_1; 
+x_1 = lean_unsigned_to_nat(324u);
+return x_1;
+}
+}
+LEAN_EXPORT lean_object* lp_LDIRProofs_List_foldl___at___00LDIR_cumWidth_spec__0(lean_object* x_1, lean_object* x_2) {
+_start:
+{
+if (lean_obj_tag(x_2) == 0)
+{
+return x_1;
+}
+else
+{
+lean_object* x_3; 
+x_3 = lean_ctor_get(x_2, 0);
+if (lean_obj_tag(x_3) == 1)
+{
+lean_object* x_4; lean_object* x_5; lean_object* x_6; 
+x_4 = lean_ctor_get(x_2, 1);
+x_5 = lean_ctor_get(x_3, 2);
+x_6 = lean_nat_add(x_1, x_5);
+lean_dec(x_1);
+x_1 = x_6;
+x_2 = x_4;
+goto _start;
+}
+else
+{
+lean_object* x_8; lean_object* x_9; lean_object* x_10; 
+x_8 = lean_ctor_get(x_2, 1);
+x_9 = lean_ctor_get(x_3, 0);
+x_10 = lean_nat_add(x_1, x_9);
+lean_dec(x_1);
+x_1 = x_10;
+x_2 = x_8;
+goto _start;
+}
+}
+}
+}
+LEAN_EXPORT lean_object* lp_LDIRProofs_List_foldl___at___00LDIR_cumWidth_spec__0___boxed(lean_object* x_1, lean_object* x_2) {
+_start:
+{
+lean_object* x_3; 
+x_3 = lp_LDIRProofs_List_foldl___at___00LDIR_cumWidth_spec__0(x_1, x_2);
+lean_dec(x_2);
+return x_3;
+}
+}
+static lean_object* _init_lp_LDIRProofs_LDIR_cumWidth___closed__0(void) {
+_start:
+{
+lean_object* x_1; lean_object* x_2; 
+x_1 = lean_unsigned_to_nat(0u);
+x_2 = lean_mk_empty_array_with_capacity(x_1);
+return x_2;
+}
+}
+LEAN_EXPORT lean_object* lp_LDIRProofs_LDIR_cumWidth(lean_object* x_1, lean_object* x_2) {
+_start:
+{
+lean_object* x_3; lean_object* x_4; lean_object* x_5; lean_object* x_6; 
+x_3 = lean_unsigned_to_nat(0u);
+x_4 = lean_obj_once(&lp_LDIRProofs_LDIR_cumWidth___closed__0, &lp_LDIRProofs_LDIR_cumWidth___closed__0_once, _init_lp_LDIRProofs_LDIR_cumWidth___closed__0);
+lean_inc(x_1);
+x_5 = l___private_Init_Data_List_Impl_0__List_takeTR_go___redArg(x_1, x_1, x_2, x_4);
+lean_dec(x_1);
+x_6 = lp_LDIRProofs_List_foldl___at___00LDIR_cumWidth_spec__0(x_3, x_5);
+lean_dec(x_5);
+return x_6;
+}
+}
+LEAN_EXPORT uint8_t lp_LDIRProofs_LDIR_feasibleBreak(lean_object* x_1, lean_object* x_2, lean_object* x_3) {
+_start:
+{
+lean_object* x_4; 
+if (lean_obj_tag(x_3) == 0)
+{
+lean_object* x_11; 
+x_11 = lean_unsigned_to_nat(0u);
+x_4 = x_11;
+goto block_10;
+}
+else
+{
+lean_object* x_12; 
+x_12 = lean_ctor_get(x_3, 0);
+lean_inc(x_12);
+lean_dec_ref(x_3);
+x_4 = x_12;
+goto block_10;
+}
+block_10:
+{
+lean_object* x_5; lean_object* x_6; lean_object* x_7; lean_object* x_8; uint8_t x_9; 
+lean_inc(x_1);
+x_5 = lp_LDIRProofs_LDIR_cumWidth(x_1, x_2);
+x_6 = lp_LDIRProofs_LDIR_cumWidth(x_1, x_4);
+x_7 = lean_nat_sub(x_5, x_6);
+lean_dec(x_6);
+lean_dec(x_5);
+x_8 = lean_unsigned_to_nat(324u);
+x_9 = lean_nat_dec_le(x_7, x_8);
+lean_dec(x_7);
+return x_9;
+}
+}
+}
+LEAN_EXPORT lean_object* lp_LDIRProofs_LDIR_feasibleBreak___boxed(lean_object* x_1, lean_object* x_2, lean_object* x_3) {
+_start:
+{
+uint8_t x_4; lean_object* x_5; 
+x_4 = lp_LDIRProofs_LDIR_feasibleBreak(x_1, x_2, x_3);
+x_5 = lean_box(x_4);
+return x_5;
+}
+}
+static lean_object* _init_lp_LDIRProofs_LDIR_demeritsReal___closed__0(void) {
+_start:
+{
+lean_object* x_1; lean_object* x_2; 
+x_1 = lean_unsigned_to_nat(10000u);
+x_2 = lean_nat_to_int(x_1);
+return x_2;
+}
+}
+LEAN_EXPORT lean_object* lp_LDIRProofs_LDIR_demeritsReal(lean_object* x_1, lean_object* x_2, lean_object* x_3) {
+_start:
+{
+uint8_t x_4; 
+x_4 = lp_LDIRProofs_LDIR_feasibleBreak(x_1, x_2, x_3);
+if (x_4 == 0)
+{
+lean_object* x_5; 
+x_5 = lean_obj_once(&lp_LDIRProofs_LDIR_demeritsReal___closed__0, &lp_LDIRProofs_LDIR_demeritsReal___closed__0_once, _init_lp_LDIRProofs_LDIR_demeritsReal___closed__0);
+return x_5;
+}
+else
+{
+lean_object* x_6; 
+x_6 = lean_obj_once(&lp_LDIRProofs_LDIR_instReprKPItem_repr___closed__11, &lp_LDIRProofs_LDIR_instReprKPItem_repr___closed__11_once, _init_lp_LDIRProofs_LDIR_instReprKPItem_repr___closed__11);
+return x_6;
+}
+}
+}
+LEAN_EXPORT lean_object* lp_LDIRProofs___private_LDIRProofs_ProofLayoutProperties_0__LDIR_instReprKPItem_repr_match__1_splitter___redArg(lean_object* x_1, lean_object* x_2, lean_object* x_3, lean_object* x_4) {
+_start:
+{
+switch (lean_obj_tag(x_1)) {
+case 0:
+{
+lean_object* x_5; lean_object* x_6; 
+lean_dec(x_4);
+lean_dec(x_3);
+x_5 = lean_ctor_get(x_1, 0);
+lean_inc(x_5);
+lean_dec_ref(x_1);
+x_6 = lean_apply_1(x_2, x_5);
+return x_6;
+}
+case 1:
+{
+lean_object* x_7; lean_object* x_8; lean_object* x_9; lean_object* x_10; 
+lean_dec(x_4);
+lean_dec(x_2);
+x_7 = lean_ctor_get(x_1, 0);
+lean_inc(x_7);
+x_8 = lean_ctor_get(x_1, 1);
+lean_inc(x_8);
+x_9 = lean_ctor_get(x_1, 2);
+lean_inc(x_9);
+lean_dec_ref(x_1);
+x_10 = lean_apply_3(x_3, x_7, x_8, x_9);
+return x_10;
+}
+default: 
+{
+lean_object* x_11; lean_object* x_12; uint8_t x_13; lean_object* x_14; lean_object* x_15; 
+lean_dec(x_3);
+lean_dec(x_2);
+x_11 = lean_ctor_get(x_1, 0);
+lean_inc(x_11);
+x_12 = lean_ctor_get(x_1, 1);
+lean_inc(x_12);
+x_13 = lean_ctor_get_uint8(x_1, sizeof(void*)*2);
+lean_dec_ref(x_1);
+x_14 = lean_box(x_13);
+x_15 = lean_apply_3(x_4, x_11, x_12, x_14);
+return x_15;
+}
+}
+}
+}
+LEAN_EXPORT lean_object* lp_LDIRProofs___private_LDIRProofs_ProofLayoutProperties_0__LDIR_instReprKPItem_repr_match__1_splitter(lean_object* x_1, lean_object* x_2, lean_object* x_3, lean_object* x_4, lean_object* x_5) {
+_start:
+{
+switch (lean_obj_tag(x_2)) {
+case 0:
+{
+lean_object* x_6; lean_object* x_7; 
+lean_dec(x_5);
+lean_dec(x_4);
+x_6 = lean_ctor_get(x_2, 0);
+lean_inc(x_6);
+lean_dec_ref(x_2);
+x_7 = lean_apply_1(x_3, x_6);
+return x_7;
+}
+case 1:
+{
+lean_object* x_8; lean_object* x_9; lean_object* x_10; lean_object* x_11; 
+lean_dec(x_5);
+lean_dec(x_3);
+x_8 = lean_ctor_get(x_2, 0);
+lean_inc(x_8);
+x_9 = lean_ctor_get(x_2, 1);
+lean_inc(x_9);
+x_10 = lean_ctor_get(x_2, 2);
+lean_inc(x_10);
+lean_dec_ref(x_2);
+x_11 = lean_apply_3(x_4, x_8, x_9, x_10);
+return x_11;
+}
+default: 
+{
+lean_object* x_12; lean_object* x_13; uint8_t x_14; lean_object* x_15; lean_object* x_16; 
+lean_dec(x_4);
+lean_dec(x_3);
+x_12 = lean_ctor_get(x_2, 0);
+lean_inc(x_12);
+x_13 = lean_ctor_get(x_2, 1);
+lean_inc(x_13);
+x_14 = lean_ctor_get_uint8(x_2, sizeof(void*)*2);
+lean_dec_ref(x_2);
+x_15 = lean_box(x_14);
+x_16 = lean_apply_3(x_5, x_12, x_13, x_15);
+return x_16;
+}
+}
+}
+}
 lean_object* initialize_Init(uint8_t builtin);
 lean_object* initialize_mathlib_Mathlib_Data_List_Basic(uint8_t builtin);
 lean_object* initialize_mathlib_Mathlib_Data_List_Lemmas(uint8_t builtin);
@@ -1122,6 +1384,8 @@ lean_dec_ref(res);
 res = initialize_LDIRProofs_LDIRProofs_proof__ir__wellformedness(builtin);
 if (lean_io_result_is_error(res)) return res;
 lean_dec_ref(res);
+lp_LDIRProofs_LDIR_lineWidth = _init_lp_LDIRProofs_LDIR_lineWidth();
+lean_mark_persistent(lp_LDIRProofs_LDIR_lineWidth);
 return lean_io_result_mk_ok(lean_box(0));
 }
 #ifdef __cplusplus
